...

HouLean/Meta/SpecializeAndSimp/Types.lean
@@ -15,22 +15,57 @@ structure Config where
 
 structure Context where
   config : Config := {}
-  skipSpecialization : Expr → MetaM Bool := fun _ => pure false
 
 structure State where
   specializations : ExprMap Specialization := {}
+  specOrder : Array Name := {}
 
-abbrev M := ReaderT Context <| StateT State SimpM
+private opaque MethodsRefPointed : NonemptyType.{0}
+def MethodsRef : Type := MethodsRefPointed.type
+instance : Nonempty MethodsRef :=
+  by exact MethodsRefPointed.property
+
+abbrev M := ReaderT MethodsRef <| ReaderT Context <| StateT State SimpM
 
 instance : MonadRecDepth M where
-  withRecDepth n x := fun ctx s => MonadRecDepth.withRecDepth n (x ctx s)
+  withRecDepth n x := fun mthds ctx s => MonadRecDepth.withRecDepth n (x mthds ctx s)
   getRecDepth := liftM (m := SimpM) <| MonadRecDepth.getRecDepth
   getMaxRecDepth := liftM (m := SimpM) <| MonadRecDepth.getMaxRecDepth
+
+
+-- forward declare `specializeExpr`
+initialize specializeExprRef : IO.Ref (Expr → M Expr) ← IO.mkRef (fun e => pure e)
+def specializeExpr (e : Expr) : M Expr := do
+  (← specializeExprRef.get) e
 
 -- forward declare `specializeAndSimp`
 initialize specializeAndSimpRef : IO.Ref (Expr → M Expr) ← IO.mkRef (fun e => pure e)
 def specializeAndSimp (e : Expr) : M Expr := do
   (← specializeAndSimpRef.get) e
+
+
+structure Methods where
+  spec : Expr → M (Option Expr) := fun _ => return none
+deriving Inhabited
+
+unsafe def Methods.toMethodsRefImpl (m : Methods) : MethodsRef :=
+  unsafeCast m
+
+@[implemented_by Methods.toMethodsRefImpl]
+opaque Methods.toMethodsRef (m : Methods) : MethodsRef
+
+unsafe def MethodsRef.toMethodsImpl (m : MethodsRef) : Methods :=
+  unsafeCast m
+
+@[implemented_by MethodsRef.toMethodsImpl]
+opaque MethodsRef.toMethods (m : MethodsRef) : Methods
+
+def getMethods : M Methods :=
+  return MethodsRef.toMethods (← read)
+
+/-- Run customizable specialization function. -/
+def customSpec (e : Expr) : M (Option Expr) := do
+  (← getMethods).spec e
 
 
 def getTheorems (attr : Name) : MetaM SimpTheorems := do
@@ -59,22 +94,26 @@ simproc_decl let_stopper_simproc (_) := fun e => do
 def M.runInMeta (x : M α)
    (config : Config := {}) (simpConfig : Simp.Config := {})
    (simpAttrs : Array Name := #[])
-   (skipSpec : Expr → MetaM Bool) : MetaM α := do
+   (customSpec : Expr → M (Option Expr)) : MetaM α := do
 
   let ctx : SpecializeAndSimp.Context := {
     config := config,
-    skipSpecialization := skipSpec
   }
   let s : SpecializeAndSimp.State := {}
+  let mthds : MethodsRef := {
+      spec := customSpec
+      : Methods
+    }.toMethodsRef
 
-  -- todo: always include `let_stopper_simproc`
-  let simpMthds := Simp.mkDefaultMethodsCore (← simpAttrs.mapM getSimprocs)
   let simpCtx : Simp.Context ← Simp.mkContext
     (config := simpConfig)
     (simpTheorems := ← simpAttrs.mapM getTheorems)
   let simpState : Simp.State := {}
+  -- todo: always include `let_stopper_simproc`
+  let simpMthds := Simp.mkDefaultMethodsCore (← simpAttrs.mapM getSimprocs)
 
-  let ((r, _), _) ← x ctx s simpMthds.toMethodsRef simpCtx |>.run simpState
+  let ((r, _), _) ← x mthds ctx s simpMthds.toMethodsRef simpCtx |>.run simpState
+
   return r
 
 
@@ -82,21 +121,7 @@ end SpecializeAndSimp
 
 open SpecializeAndSimp in
 def specializeAndSimp (e : Expr)
-     (config : SpecializeAndSimp.Config := {}) (simpConfig : Simp.Config := {})
-     (simpAttrs : Array Name := #[])
-     (skipSpec : Expr → MetaM Bool) : MetaM Expr := do
-  (SpecializeAndSimp.specializeAndSimp e).runInMeta config simpConfig simpAttrs skipSpec
-
-
-
--- skip specialization based in implemented_by
-  -- -- has implemented by
-  -- -- we have to really check unification as function like `getElem` might have few implemented_by
-  -- -- but in most cases we want to specialize it
-  -- let s := (compilerExt.getState (← getEnv)).implementedBy
-  -- let candidates ← s.getMatch e
-  -- for c in candidates do
-  --   let (xs,_,_) ← forallMetaTelescope (← inferType c.lhs)
-  --   let b := c.lhs.beta xs
-  --   if ← isDefEq e b then
-  --     return .true
+    (config : SpecializeAndSimp.Config := {}) (simpConfig : Simp.Config := {})
+    (simpAttrs : Array Name := #[])
+    (customSpec : Expr → M (Option Expr) := fun _ => return none) : MetaM Expr := do
+  (SpecializeAndSimp.specializeAndSimp e).runInMeta config simpConfig simpAttrs customSpec
