Tests/Meta/SpecAndSimp.lean
@@ -1,5 +1,7 @@
 import HouLean.Meta.SpecializeAndSimp.Main
 import HouLean.OpenCL.Basic
+-- import HouLean.OpenCL.Data.Fin
+import HouLean.OpenCL.Data.InlinedLoop
 import HouLean.OpenCL.Reference.Operators
 import HouLean.Data.Matrix
 import HouLean.Data.Vector
@@ -11,25 +13,37 @@ open Lean Meta Qq HouLean Meta
 
 namespace Test.OpenCL.SpecAndSimp
 
-open OpenCL.Compiler3
-def skipImplementedBy (e : Expr) : MetaM Bool := do
+
+open OpenCL.Compiler3 SpecializeAndSimp in
+def specializeImplementedBy (e : Expr) : M (Option Expr) := do
   let s := (compilerExt.getState (← getEnv)).implementedBy
   let candidates ← s.getMatch e
   for c in candidates do
     let (xs,_,_) ← forallMetaTelescope (← inferType c.lhs)
+
+    -- is 'implemented_by' applicable?
+    -- we have to go over all arguments and check if they really apply/classes have instances
     let b := c.lhs.beta xs
     if ← isDefEq e b then
       let mut skip := false
       for x in xs do
+        let x ← instantiateMVars x
         let t ← inferType x
-        if (← isClass? t).isSome then
-          if (← synthInstance? t).isNone then
+        if (← isClass? t).isSome && x.isMVar then
+          if let some inst ← synthInstance? t then
+            x.mvarId!.assign inst
+          else
             skip := true
+            break
       if skip then
         continue
-      -- logInfo m!"skipping specialization of {e}"
-      return true
-  return false
+
+      let xs' ← xs.mapM specializeExpr
+      let e' := c.lhs.beta xs'
+      -- logInfo m!"{xs} ==> {xs'}"
+      -- logInfo m!"custom spec{indentExpr e}==>{indentExpr e'}"
+      return e'
+  return none
 
 
 def foo {α} [Add α] [Mul α] (x : α) :=
@@ -41,7 +55,42 @@ def foo {α} [Add α] [Mul α] (x : α) :=
 
 #eval foo 10
 
-attribute [opencl_csimp] Nat.add_zero Nat.zero_add
+/-- Gadget identity map that will unroll loops at compile time. -/
+def unroll {α : Sort u} (a : α) : α := a
+
+def evalNat' (e : Expr) : MetaM (Option Nat) := do
+  try
+    let n ← unsafe evalExpr' Nat ``Nat e
+    return some n
+  catch _ =>
+    return none
+
+simproc_decl list_ofFn_unroll (unroll (List.ofFn _)) := fun e => do
+  let e ← instantiateMVars e.appArg!
+  if let some (t, n, f) := e.app3? ``List.ofFn then
+    if let some n ← evalNat' n then
+      let mut e ← mkAppOptM ``List.nil #[t]
+      for h : i in [0:n] do
+        have ⟨_,_⟩ := h
+        let i : Fin n := ⟨n-i-1, by grind⟩
+        let i := toExpr i
+        e ← mkAppM ``List.cons #[f.app i, e]
+      return .visit { expr := e}
+  return .continue
+
+#check (unroll <| List.ofFn (fun i : Fin 5 => 3*i.1)) rewrite_by simp only [list_ofFn_unroll]
+
+@[opencl_csimp]
+theorem vector_mk_ofFn {α : Type} {n : Nat} (f : Fin n → α) (h) :
+  Vector.mk (n:=n) (List.ofFn f).toArray h
+  =
+  Vector.mk (n:=n) (unroll (List.ofFn f)).toArray h  := sorry
+
+attribute [opencl_csimp] Nat.add_zero Nat.zero_add list_ofFn_unroll
+
+#check (Vector.mk (n:=5) (List.ofFn fun i : Fin 5 => 3*i.1).toArray rfl)
+  rewrite_by
+    simp only [opencl_csimp]
 
 run_meta
   let e :=
@@ -57,22 +106,30 @@ run_meta
       a + b)
 
   lambdaTelescope e fun _ e => do
-  let e' ← specializeAndSimp e {} { zeta := false } #[`opencl_csimp] skipImplementedBy
+  let e' ← specializeAndSimp e {} { zeta := false, zetaDelta := false }
+    #[`opencl_csimp] specializeImplementedBy
 
   logInfo e'
 
-
 impl_by (x y z : Float) : #v[x,y,z] ==> (float3){x,y,z}
 
-impl_by {α : Type} (u : Vector α 3) (h : 0 < 3) : getElem u 0 h ==> u.x
-impl_by {α : Type} (u : Vector α 3) (h : 1 < 3) : u[1]'h ==> u.y
-impl_by {α : Type} (u : Vector α 3) (h : 2 < 3) : u[2]'h ==> u.z
+set_option pp.funBinderTypes true in
+-- todo: turn this into a `impl_by` rule that creates the rhs
+impl_by {α : Type} {n : Nat} (u : Vector α n) (i : Nat) (h) : getElem u i h ==> getElem(u,i)
+impl_by {α : Type} {n : Nat} (u : Vector α n) (i : Fin n) (h) : getElem u i (h) ==> getElem(u,i)
 
 @[opencl_csimp]
 theorem vector_map (v : Vector α n) (f : α → β) : v.map f = .ofFn (fun i => f v[i]) := sorry_proof
 
 @[opencl_csimp]
-theorem vector_ofFn (f : Fin 3 → α) : Vector.ofFn f = #v[f 0, f 1, f 2] := sorry_proof
+theorem vector_mapFinIdx (v : Vector α n) (f : (i : Nat) → α → (h : i < n) → β) :
+  v.mapFinIdx f = .ofFn (fun i => f i.1 v[i.1] i.2) := sorry_proof
+
+@[opencl_csimp]
+theorem inline_foldl (f : α → Fin n → α) (init : α) :
+  Fin.foldl n f init
+  =
+  OpenCL.inlinedLoop n (fun i s => f s i) init := sorry_proof
 
 
 -- variable (x : Vector Float 3)
@@ -81,11 +138,66 @@ macro_rules | `(tactic| get_elem_tactic_extensible) => `(tactic| sorry_proof)
 
 
 -- set_option trace.HouLean.specialize.detail true
--- run_meta
---   let e :=
---     q(fun x y z : Float => #v[x,y,z])
+run_meta
+  let e :=
+    q(fun x y z : Float =>
+        let a := foo x
+        let b := y
+        let c := foo (z + foo x)
+        #v[a, b, c])
 
---   lambdaTelescope e fun _ e => do
---   let e' ← specializeAndSimp e {} { zeta := false } #[`opencl_csimp] skipImplementedBy
+  lambdaTelescope e fun _ e => do
+  let e' ← specializeAndSimp e {} { zeta := false } #[`opencl_csimp] specializeImplementedBy
 
---   logInfo e'
+  logInfo e'
+
+
+set_option trace.HouLean.specialize true
+run_meta
+  let e :=
+    q(fun x : Vector Float 3 => x * x)
+
+  lambdaTelescope e fun _ e => do
+  let e' ← specializeAndSimp e {} { zeta := false } #[`opencl_csimp] specializeImplementedBy
+  logInfo e'
+
+set_option trace.HouLean.specialize true
+run_meta
+  let e :=
+    q(fun x : Vector Float 3 => x[0])
+
+  lambdaTelescope e fun _ e => do
+  let e' ← specializeAndSimp e {} { zeta := false } #[`opencl_csimp] specializeImplementedBy
+  logInfo e'
+
+attribute [opencl_csimp] sum Fin.getElem_fin
+
+@[opencl_csimp]
+theorem Float.zero_add (x : Float) : 0 + x = x := sorry_proof
+
+@[opencl_csimp]
+theorem Float.add_zero (x : Float) : x + 0 = x := sorry_proof
+
+
+set_option trace.HouLean.specialize true
+set_option pp.proofs false
+set_option trace.Meta.Tactic.simp.rewrite true in
+run_meta
+  let e :=
+    q(fun x : Vector Float 3 => x.dot x)
+
+  lambdaTelescope e fun _ e => do
+  let e' ← specializeAndSimp e {} { zeta := false } #[`opencl_csimp] specializeImplementedBy
+  logInfo e'
+
+
+#check isRecursiveDefinition
+set_option trace.HouLean.specialize true
+run_meta
+  let e :=
+    q(fun x : Matrix Float 3 3 => x + x)
+
+  lambdaTelescope e fun _ e => do
+  let e' ← specializeAndSimp e {} { zeta := false } #[`opencl_csimp] specializeImplementedBy
+
+  logInfo e'
