HouLean/OpenCL/Compiler/RewriteRules.lean
@@ -39,7 +39,8 @@ deriving Inhabited, BEq
 structure ImplementedByBuilder where
   keys : Array DiscrTree.Key
   lhs : Expr
-  syntaxBuilder : Name
+  declName : Name
+  arity : Nat
 deriving Inhabited, BEq
 
 inductive SingleExtension where
@@ -109,6 +110,37 @@ partial def implementedBy (e : Expr) : MetaM (TSyntax `oclExpr) := do
 
    throwError "Don't know how to compile {e}!"
 
+
+open Lean Meta
+def addImpementedBy (lhs : Expr) (rhs : TSyntax `oclExpr) : MetaM Unit := do
+  let type ← inferType lhs
+
+  -- figure out which arguments of lhs appear on the rhs
+  -- store their name and index
+  let argsToCompile ←
+    forallTelescope type fun args _ => do
+      args.zip (.range args.size)
+        |>.filterMapM (fun (arg,i) => do
+          if arg.isFVar then
+            let name ← arg.fvarId!.getUserName
+            -- arguments that appear on the rhs should be compiled!
+            if rhs.raw.hasIdent name then
+              return some (name, i)
+          return none)
+
+  let (xs,_,_) ← forallMetaTelescope (← inferType lhs)
+  let body := lhs.beta xs
+  let keys ← DiscrTree.mkPath body
+
+  let impl : ImplementedBy := {
+    keys := keys
+    argsToCompile := argsToCompile
+    lhs := lhs
+    rhs := rhs
+  }
+
+  compilerExt.add (.implementedBy impl)
+
 open Lean Elab Term Command
 elab "impl_by" bs:bracketedBinder* " : " lhs:term  " ==> " rhs:oclExpr : command => do
 
@@ -122,35 +154,11 @@ elab "impl_by" bs:bracketedBinder* " : " lhs:term  " ==> " rhs:oclExpr : command
       let e ← mkLambdaFVars ctx' e >>= instantiateMVars
 
       if e.hasMVar || e.hasFVar then
-        throwError s!"Bug in {decl_name%}, failed to build lhs expression!"
+        let fvars := (← e.collectFVars.run {}).2.fvarIds.map Expr.fvar
+        let mvars := (e.collectMVars {}).result.map (Expr.mvar)
+        throwError s!"Bug in {decl_name%}, failed to build lhs expression! fvars: {fvars}, mvars: {mvars}, {e} : {← inferType e}"
 
-      let args := ctx' ++ xs
-      -- collect identifiers that appear on the rhs
-      let argsToCompile : Array (Name × Nat) ←
-        (args.zip (.range args.size))
-        |>.filterMapM (fun (arg,i) => do
-          if arg.isFVar then
-            let name ← arg.fvarId!.getUserName
-            if rhs.raw.hasIdent name then
-              return some (name, i)
-          return none)
-
-      -- todo: add tracing
-      -- logInfo m!"lhs: {e}\nargs to compile: {argsToCompile}"
-
-      let (_,_,body) ← lambdaMetaTelescope e
-      let keys ← DiscrTree.mkPath body
-
-      -- let declName ← mkUniqueDeclName `implBy
-
-      let impl : ImplementedBy := {
-        keys := keys
-        argsToCompile := argsToCompile
-        lhs := e
-        rhs := rhs
-      }
-
-      compilerExt.add (.implementedBy impl)
+      addImpementedBy e rhs
 
 
 open Lean Elab Term Command Qq
@@ -192,8 +200,44 @@ elab "impl_by" bs:bracketedBinder* " : " lhs:term  " ==> " "do" rhs:doElem* : co
       let b : ImplementedByBuilder := {
         keys := keys
         lhs := e
-        syntaxBuilder := builderDeclName
+        declName := builderDeclName
+        arity := decls.size
       }
 
       compilerExt.add (.implementedByBuilder b)
       logInfo m!"script:\n{rhs}"
+
+
+#check Simp.getSimprocExtension?
+
+  -- let ctx ← read
+  -- match ctx.env.find? declName with
+  -- | none      => throw <| IO.userError ("Unknown constant `" ++ toString declName ++ "`")
+  -- | some info =>
+  --   match info.type with
+  --   | .const ``Simproc _ =>
+  --     return .inl (← IO.ofExcept <| ctx.env.evalConst Simproc ctx.opts declName)
+  --   | .const ``DSimproc _ =>
+  --     return .inr (← IO.ofExcept <| ctx.env.evalConst DSimproc ctx.opts declName)
+  --   | _ => throw <| IO.userError s!"Simproc `{privateToUserName declName}` has an unexpected type: Expected `Simproc` or `DSimproc`, but found `{info.type}`"
+
+
+unsafe def getBuilder (declName : Name) : CoreM (Array Expr → MetaM (TSyntax `oclExpr)) := do
+  let env ← getEnv
+  let opts ← getOptions
+  match env.find? declName with
+  | none      => throwError m!"Unknown constant `{declName}`"
+  | some info =>
+    match info.type with
+    | .const ``ImplementedByBuilder _ =>
+      return (← IO.ofExcept <| env.evalConst (Array Expr → MetaM (TSyntax `oclExpr)) opts declName)
+    | _ => throwError m!"ImplementedByBuilder `{privateToUserName declName}` has an unexpected type: Expected `ImplementedByBuilder`, but found `{info.type}`"
+
+
+def instantiateBuilder (xs : Array Expr) (builder : ImplementedByBuilder) : MetaM Bool := do
+
+  let lhs := builder.lhs.beta xs
+  let b ← unsafe getBuilder builder.declName
+  let rhs ← b xs
+
+  sorry
