HouLean/OpenCL/Reference/VectorComponentAndConstructor.lean
@@ -1,0 +1,127 @@
+import HouLean.OpenCL.Compiler.RewriteRules
+
+open HouLean OpenCL Compiler Math
+
+namespace HouLean.OpenCL
+
+variable {α : Type} [AtomicOpenCLType α] {n : Nat}
+
+-- todo: to changes to explicit projections .x, .y, .z, .w, .s4, .s5, ...
+impl_by {α : Type} [AtomicOpenCLType α] {n : Nat} (u : Vector α n) (i : Nat) (h) :
+    getElem u i h ==> getElem(u,i)
+
+
+open Lean Meta
+def compileExpr (e : Expr) : MetaM (TSyntax `oclExpr) := sorry
+def compileType (e : Expr) : MetaM Ident := sorry
+def runInterpreter? (α : Type) (e : Expr) : MetaM (Option α) := sorry
+
+
+def indexToSuffix? (i : Nat) : Option Name :=
+  match i with
+  | 0 => `x
+  | 1 => `y
+  | 2 => `z
+  | 3 => `w
+  | 4 => `s4
+  | 5 => `s5
+  | 6 => `s6
+  | 7 => `s7
+  | 8 => `s8
+  | 9 => `s9
+  | 10 => `sa
+  | 11 => `sb
+  | 12 => `sc
+  | 13 => `sd
+  | 14 => `se
+  | 15 => `sf
+  | _ => none
+
+
+open Lean Meta in
+impl_by (u : Vector α n) (i : Nat) (h) : u[i]'h ==> do
+
+  let some i ← runInterpreter? Nat i
+    | throwError m!"Must know {i} at compile time when compiling `{u}[{i}]`"
+  let u ← compileExpr u
+
+  let some suffix := indexToSuffix? i
+    | throwError m!"Invalid index {i}, has to be smaller than 16!"
+  let idx := mkIdent suffix
+
+  return ← `(oclExpr| $u:oclExpr.$idx:ident)
+
+-- normalize `getElem` from indexing with `Fin n` to indexing with `Nat`
+attribute [opencl_csimp] Fin.getElem_fin
+
+----------------------------------------------------------------------------------------------------
+--
+
+
+#check evalConst
+
+/- Vector contructor rule  e.g. #v[x,y,z] ==> (float3){x,y,z}
+
+The notation `#v[x,y,z]` stands for `Vector.mk [x,y,z].toArray h` and this rule matches on this
+irrespective of the length of the list.
+ -/
+impl_by {α : Type} [AtomicOpenCLType α] (l : List α) (h) :
+    Vector.mk l.toArray h ==> do
+
+  let xs ← splitList l
+  let xs ← xs.mapM compileExpr
+  let t ← compileType α
+
+  return ← `(oclExpr| ($t){$xs,*} )
+
+
+-- def genericKernel
+--       {npts : Nat, dim : Nat}
+--       [FloatType R]
+--       (timeStep : R,
+--        P : Attribute .point (Vector R dim) (size := npts) (write := true),
+--        v : Attribute .point (Vector R dim) (size := npts)):
+
+--     i = getGlobalWorkId()
+--     if not (i < npts):
+--       return
+
+--     pos = P[i]
+--     P[i] += dt * v[i]
+
+
+-- vector 2
+impl_by (x y : Nat) : #v[x,y] ==> (uint3){x,y}
+impl_by (x y : Int) : #v[x,y] ==> (int3){x,y}
+impl_by (x y : UInt16) : #v[x,y] ==> (ushort3){x,y}
+impl_by (x y :  Int16) : #v[x,y] ==>  (short3){x,y}
+impl_by (x y : UInt32) : #v[x,y] ==> (uint3){x,y}
+impl_by (x y :  Int32) : #v[x,y] ==>  (int3){x,y}
+impl_by (x y : UInt64) : #v[x,y] ==> (ulong3){x,y}
+impl_by (x y :  Int64) : #v[x,y] ==>  (long3){x,y}
+impl_by (x y : Float32) : #v[x,y] ==> (float3){x,y}
+impl_by (x y : Float64) : #v[x,y] ==> (double3){x,y}
+
+-- vector 3
+impl_by (x y z : Nat) : #v[x,y,z] ==> (uint3){x,y,z}
+impl_by (x y z : Int) : #v[x,y,z] ==> (int3){x,y,z}
+impl_by (x y z : UInt16) : #v[x,y,z] ==> (ushort3){x,y,z}
+impl_by (x y z :  Int16) : #v[x,y,z] ==>  (short3){x,y,z}
+impl_by (x y z : UInt32) : #v[x,y,z] ==> (uint3){x,y,z}
+impl_by (x y z :  Int32) : #v[x,y,z] ==>  (int3){x,y,z}
+impl_by (x y z : UInt64) : #v[x,y,z] ==> (ulong3){x,y,z}
+impl_by (x y z :  Int64) : #v[x,y,z] ==>  (long3){x,y,z}
+impl_by (x y z : Float32) : #v[x,y,z] ==> (float3){x,y,z}
+impl_by (x y z : Float64) : #v[x,y,z] ==> (double3){x,y,z}
+
+-- vector 4
+impl_by (x y z w : Nat) : #v[x,y,z,w] ==> (uint4){x,y,z,w}
+impl_by (x y z w : Int) : #v[x,y,z,w] ==> (int4){x,y,z,w}
+impl_by (x y z w : UInt16) : #v[x,y,z,w] ==> (ushort4){x,y,z,w}
+impl_by (x y z w :  Int16) : #v[x,y,z,w] ==>  (short4){x,y,z,w}
+impl_by (x y z w : UInt32) : #v[x,y,z,w] ==> (uint4){x,y,z,w}
+impl_by (x y z w :  Int32) : #v[x,y,z,w] ==>  (int4){x,y,z,w}
+impl_by (x y z w : UInt64) : #v[x,y,z,w] ==> (ulong4){x,y,z,w}
+impl_by (x y z w :  Int64) : #v[x,y,z,w] ==>  (long4){x,y,z,w}
+impl_by (x y z w : Float32) : #v[x,y,z,w] ==> (float4){x,y,z,w}
+impl_by (x y z w : Float64) : #v[x,y,z,w] ==> (double4){x,y,z,w}
